classes

Classes.v
@@ -1,156 +1,166 @@
-Require Import List.
+Require Import List Bool Arith.
 Import ListNotations.
 Require Import Relations Morphisms.
+Require Import Omega.
+
+Generalizable Variables X Y.
 
 Class eqType (X : Type) : Type := eq_dec : forall x y : X, {x=y} + {x<>y}.
 
-Class Finite {X} `{eqType X} : Type := enum : {xs: list X|forall x, In x xs}.
+Instance : eqType bool := bool_dec.
+Instance : eqType nat := eq_nat_dec.
+Instance : eqType True.
+Proof. intros x y. destruct x; destruct y; auto. Qed.
+Instance : eqType False.
+Proof. intros x; destruct x. Qed.
 
-Definition test `{eqType X} := X.
+Program Instance sum_eqType `(eqType X) `(eqType Y) : eqType(X+Y) := fun a b =>
+match a, b with
+  | inl _, inr _ | inr _, inl _ => right _
+  | inl z, inl z' | inr z, inr z' =>
+      match eq_dec z z' with left _ => left _
+                           | right _ => right _
+      end
+end.
 
-Check Set.
+Program Instance prod_eqType `(eqType X) `(eqType Y) : eqType(X*Y) := fun a b =>
+match a,b with
+  | pair x y, pair x' y' =>
+  match eq_dec x x', eq_dec y y' with
+    | left _, left _ => left _
+    | left _, right _ | right _, left _ | right _, right _ => right _
+  end
+end.
 
-Check count_occ.
+Eval compute in if eq_dec ((4,3)) ((2,3)) then true else false.
 
-Program Instance : Finite := [true;false].
+Instance prod_eqType `(eqType X) `(eqType Y) : eqType(X*Y).
+
+
+Section Finite.
+
+Class Finite (X : Type) `{eqType X} : Type := enum : {xs: list X|forall x, In x xs}.
+Check Finite.
+
+Check @enum.
+Check Finite.
+
+
+Program Instance : Finite bool := [true;false].
 Next Obligation. destruct x; intuition. Qed.
 
-Program Instance : Finite := [I].
+Program Instance : Finite True := [I].
 Next Obligation. destruct x; intuition. Qed.
 
-Program Instance : @Finite False := [].
+Program Instance : Finite False := [].
 
-Eval compute in seq 0 3.
-Check length.
+Check @enum.
 
-Program Fixpoint seq' (n:nat) : {l | length l = n} := seq 0 n.
-Next Obligation. apply seq_length. Qed.
+Program Instance sum_finite `(p1:Finite X) `(p2:Finite Y) : Finite(X+Y) :=
+  (map (@inl X Y) (@enum X p1)) ++ (map (@inr X Y) (@enum Y p2)).
+Next Obligation.
+  destruct (@enum X p1) as [xs px]; destruct (@enum Y p2) as [ys py]; simpl.
+  apply in_or_app.
+  destruct x; [left|right]; apply in_map; auto.
+Qed.
 
-Program Fixpoint weaken {n:nat} (xs : list {x|x<n}) : list {x|x<S n} :=
+Program Instance prod_finite `(px: Finite X) `(py: Finite Y) : Finite(X*Y) :=
+  list_prod enum enum.
+Next Obligation.
+  destruct (@enum X px) as [xs p1]; destruct (@enum Y py) as [ys p2]; simpl.
+  auto using in_prod.
+Qed.
+
+
+
+Section Finite_Of_List.
+
+Program Definition weaken {X} {xs: list X} x (y : {y|In y xs}) : {y|In y (x::xs)} := y.
+Program Fixpoint siglist {X} (xs : list X) : list {x:X|In x xs} :=
 match xs with
   | [] => []
-  | x::xs => x :: weaken xs
+  | x::xs => x :: (map (weaken x) (siglist xs))
 end.
 
-Program Fixpoint seq'' (n:nat) : list {m|m<n} :=
-match n with
-  | O => []
-  | S n => n :: weaken (seq'' n)
+Program Instance fin_of_list {X} (xs : list X) : Finite {x|In x xs} := siglist xs.
+Next Obligation.
+  induction xs; destruct H.
+  + subst a. simpl. auto.
+  + right. 
+    assert (weaken a (exist (fun x0 : X => In x0 xs) x i) =
+            exist (fun x0 : X => In x0 (a :: xs)) x (or_intror i))
+    by auto.
+    rewrite <- H.
+    apply in_map. auto.
+Qed.
+
+End Finite_Of_List.
+
+
+
+
+
+Section Finite_Functions.
+
+Lemma 
+
+
+Program Instance fun_finite `(p1:Finite X) `(p2:Finite Y) : Finite(X->Y) :=
+ fold_right list_prod (map (list_prod (@enum Y p2)) (@enum X p1)) [].
+
+End Finite_Functions.
+
+
+
+
+
+
+
+Fixpoint power {X} (xs : list X) :=
+match xs with
+  | [] => [[]]
+  | x::xs => 
+   map (fun p => app (fst p) (snd p)) (list_prod [[x];[]] (power xs))
 end.
 
-Eval compute in map (proj1_sig _ _) (seq'' 4).
-
-Program Instance test (n:nat) : @Finite {m|m<n} := seq' n.
-
-Lemma ex : @Finite bool.
-Proof. intuition. Qed.
-
-Class Finite (X:Set) : Type := {
-  enumeration : list X;
-  enumerate : forall x : X, In x enumeration
-}.
-
-Class SemiGroup (G : Type) (e : relation G) (op : G -> G -> G) : Prop := {
-  sg_setioid : Equivalence e;
-  sg_proper : Proper (e ==> e ==> e) op
-}.
+Definition insertn {X} (n:nat) (x:X) (xs:list X) := app (firstn n xs) (x::skipn n xs).
 
 
-}
+Lemma in_insertn X (x:X) y n xs : 
+  In x xs \/ x=y -> In x (insertn n y xs).
+Proof.
+  intro H.
+  unfold insertn. apply in_or_app.
+  destruct H as [H|H].
+  + rewrite <- (firstn_skipn n) in H. apply in_app_or in H.
+    destruct H; [left|right]; simpl; auto.
+  + right. simpl. auto.
+Qed.
 
-Theorem example `{Finite X} : enumeration = enumeration.
+Fixpoint power {X} (xs : list X) :=
+match xs with
+  | [] => [[]]
+  | x::xs => flat_map f (power xs)
 
-Print X.
+Lemma in_power
 
-Parameter F : Finite.
+Program Instance list_finite `(p: Finite X) : Finite(list X) :=
+
+End Finite.
+
+Check Finite (sum (prod bool True) False).
+
 
 Class FinTy : Type := {
-  X :> Set;
-  Y : Finite(X)
+  T :> Type;
+  T_finite :> Finite T
 }.
 
-Coercion (Finite X) >-> X.
+Definition test `(FinTy) := enum.
 
-Parameter A : FinTy.
+Check test.
 
-Program Fixpoint weaken {n} (xs : list {m|m<n}) : list {m|m<S n} :=
-match xs with
-  | [] => []
-  | x::xs => x :: weaken xs
-end.
+Parameter X : FinTy.
 
-Eval compute in weaken [].
-
-Check enumeration.
-Print enumeration.
-
-Check X.
-Parameter p : Finite X.
-Print p.
-
-Check @enumeration.
-
-Program Instance prod_finite {X} {Y} (p1: Finite X) (p2: Finite Y) : Finite(X*Y) :=
-{| enumeration := (map (@inl X Y) (@enumeration(X)(p1))) ++ 
-                  (map (@inr X Y) (@enumeration(Y)(p2)));
-   enumerate := _ |}.
-
-Next Obligation.
-
-Instance sum_finite : Finite'-> Finite' -> Finite'.
-Proof.
-  intros.
-  destruct X0 as [X xs p]; destruct X1 as [Y ys p'].
-  esplit.
-  eapply p.
-  destruct H as [xs p]; destruct H0 as [ys p'].
-  econstructor; intros.
-  cut (In x (app (map inl xs) (map inr ys))); eauto.
-  apply in_or_app.
-  destruct x; [left|right]; apply in_map; auto.
-Qed.
-
-Instance sum_finite {X} {Y} : Finite X -> Finite Y -> Finite(X+Y).
-Proof.
-  intros.
-  destruct H as [xs p]; destruct H0 as [ys p'].
-  econstructor; intros.
-  cut (In x (app (map inl xs) (map inr ys))); eauto.
-  apply in_or_app.
-  destruct x; [left|right]; apply in_map; auto.
-Qed.
-
-Check sum_finite.
-
-Instance prod_finite {X} {Y} : Finite X -> Finite Y -> Finite(X*Y).
-Proof.
-  intros.
-  destruct H as [xs p]; destruct H0 as [ys p'].
-  econstructor. intros. destruct x.
-  cut (In (x,y) (list_prod xs ys)); eauto using in_prod.
-Qed.
-
-Inductive finTy {X : Set} (xs : list X) : Set :=
-  | finTyE : forall x, In x xs -> finTy xs.
-Hint Constructors finTy.
-
-Inductive atom : Set := Atom.
-
-Instance atom_finite : Finite atom.
-Proof.
-  assert(forall x : atom, In x [Atom]); econstructor; eauto.
-  destruct x; trivial.
-Qed.
-
-Inductive null : Set :=.
-Instance null_finite : Finite null.
-Proof.
-  assert(forall x : null, In x []).
-  + intro x; inversion x.
-  + econstructor; eapply H.
-Qed.
-
-Fixpoint nary (n : nat) : Finite _ :=
-match n with
-  | O -> null
-  | _
+Check T.
+Check @enum X.
