Misc.v
@@ -30,3 +30,14 @@ Proof.
   inversion H.
   split; reflexivity.
 Qed.
+
+Lemma list_eq_dec {X} (eq : forall x y:X, {x=y}+{x<>y}) (xs ys : list X) :
+  {xs=ys}+{xs<>ys}.
+Proof.
+  pose (eqb := fun x y => if eq x y then true else false).
+  assert (forall x y, eqb x y = true <-> x = y).
+  + intros. subst eqb. split; intro H;
+    simpl in H; destruct (eq x y); auto; inversion H.
+  + assert (H' := list_eqb_eq eqb H xs ys).
+    destruct (list_eqb eqb xs ys); [left|right]; intuition.
+Qed.
